Proof yields <-> reorderings.

Reorderings.v
@@ -1,4 +1,5 @@
-Require Import InfixGrammar.
+Require Import PosTree.
+Require Import PosTreeTheorems.
 From stdpp Require Import list.
 From stdpp Require Import relations.
 
@@ -9,6 +10,7 @@ Implicit Types l : L.
 Implicit Types o : O.
 Implicit Types s : L + O.
 Implicit Types t : @parse_tree L O.
+Implicit Types pt : @pos_tree L O.
 
 Inductive reorder_step : parse_tree -> parse_tree -> Prop :=
   | RI_LR t11 o1 t12 o t2 :
@@ -35,3 +37,297 @@ Proof.
   - rewrite IHreorder_step. reflexivity.
   - rewrite IHreorder_step. reflexivity.
 Qed.
+
+Lemma reorder_preserves_yield t t' :
+  reorder t t' -> yield t = yield t'.
+Proof.
+  unfold reorder. intros.
+  induction H.
+  - reflexivity.
+  - rewrite <- IHrtc.
+    apply reorder_step_preserves_yields.
+    assumption.
+Qed.
+
+Inductive reorder_step_pos : pos_tree -> pos_tree -> Prop :=
+  | PRI_LR pt11 o1 i1 pt12 o i pt2 :
+      reorder_step_pos (PINode (PINode pt11 o1 i1 pt12) o i pt2)
+                       (PINode pt11 o1 i1 (PINode pt12 o i pt2))
+  | PRI_RL pt1 o i pt21 o2 i2 pt22 :
+      reorder_step_pos (PINode pt1 o i (PINode pt21 o2 i2 pt22))
+                      (PINode (PINode pt1 o i pt21) o2 i2 pt22)
+  | PRI_pt1 pt1 o i pt2 pt1' :
+      reorder_step_pos pt1 pt1' ->
+      reorder_step_pos (PINode pt1 o i pt2) (PINode pt1' o i pt2)
+  | PRI_pt2 pt1 o i pt2 pt2' :
+      reorder_step_pos pt2 pt2' ->
+      reorder_step_pos (PINode pt1 o i pt2) (PINode pt1 o i pt2').
+
+Definition reorder_pos := rtc reorder_step_pos.
+
+Lemma reorder_step_pos_symmetry pt1 pt2 :
+  reorder_step_pos pt1 pt2 -> reorder_step_pos pt2 pt1.
+Proof.
+  intros.
+  induction H.
+  - apply PRI_RL.
+  - apply PRI_LR.
+  - apply PRI_pt1.
+    assumption.
+  - apply PRI_pt2.
+    assumption.
+Qed.
+
+Lemma reorder_pos_symmetry pt1 pt2 :
+  reorder_pos pt1 pt2 -> reorder_pos pt2 pt1.
+Proof.
+  intros.
+  induction H.
+  - apply rtc_refl.
+  - apply reorder_step_pos_symmetry in H.
+    eapply rtc_transitive.
+    + apply IHrtc.
+    + eapply rtc_l.
+      * eassumption.
+      * apply rtc_refl.
+Qed.
+
+Lemma reorder_step_pos_wf_pos_tree n0 pt n pt' :
+  wf_pos_tree n0 pt n -> reorder_step_pos pt pt' -> wf_pos_tree n0 pt' n.
+Proof.
+  intros. revert H. revert n0 n.
+  induction H0; intros.
+  - inv H. inv H6.
+    eauto with pos_tree.
+  - inv H. inv H7.
+    eauto with pos_tree.
+  - inv H.
+    eauto with pos_tree.
+  - inv H.
+    eauto with pos_tree.
+Qed.
+
+Lemma reorder_pos_wf_pos_tree n0 pt n pt' :
+  wf_pos_tree n0 pt n -> reorder_pos pt pt' -> wf_pos_tree n0 pt' n.
+Proof.
+  intros. revert H.
+  induction H0; eauto using reorder_step_pos_wf_pos_tree.
+Qed.
+
+Lemma reorder_step_pos_preserves_position pt pt' :
+  reorder_step_pos pt pt' -> pos_equivalent pt pt'.
+Proof.
+  intros. unfold pos_equivalent.
+  induction H; intros.
+  - split; intros.
+    + inv H; eauto with pos_tree.
+      inv H2; eauto with pos_tree.
+    + inv H; eauto with pos_tree.
+      inv H2; eauto with pos_tree.
+  - split; intros.
+    + inv H; eauto with pos_tree.
+      inv H2; eauto with pos_tree.
+    + inv H; eauto with pos_tree.
+      inv H2; eauto with pos_tree.
+  - split; intros.
+    + inv H0; eauto with pos_tree.
+      apply IHreorder_step_pos in H3.
+      eauto with pos_tree.
+    + inv H0; eauto with pos_tree.
+      apply IHreorder_step_pos in H3.
+      eauto with pos_tree.
+  - split; intros.
+    + inv H0; eauto with pos_tree.
+      apply IHreorder_step_pos in H3.
+      eauto with pos_tree.
+    + inv H0; eauto with pos_tree.
+      apply IHreorder_step_pos in H3.
+      eauto with pos_tree.
+Qed.
+
+Lemma reorder_pos_preserves_position pt pt' :
+  reorder_pos pt pt' -> pos_equivalent pt pt'.
+Proof.
+  intros.
+  induction H.
+  - unfold pos_equivalent.
+    auto.
+  - apply reorder_step_pos_preserves_position in H.
+    unfold pos_equivalent in *.
+    intros.
+    split; intros.
+    + apply IHrtc. apply H. assumption.
+    + apply H. apply IHrtc. assumption.
+Qed.
+
+Lemma reorder_pos_subtree_l pt1 o i pt2 pt1' :
+  reorder_pos pt1 pt1' ->
+  reorder_pos (PINode pt1 o i pt2) (PINode pt1' o i pt2).
+Proof.
+  intros.
+  induction H.
+  - apply rtc_refl.
+  - eapply rtc_l.
+    + apply PRI_pt1.
+      eassumption.
+    + assumption.
+Qed.
+
+Lemma reorder_pos_subtree_r pt1 o i pt2 pt2' :
+  reorder_pos pt2 pt2' ->
+  reorder_pos (PINode pt1 o i pt2) (PINode pt1 o i pt2').
+Proof.
+  intros.
+  induction H.
+  - apply rtc_refl.
+  - eapply rtc_l.
+    + apply PRI_pt2.
+      eassumption.
+    + assumption.
+Qed.
+
+Lemma reorder_pos_nth_op_top i o pt :
+  nth_symbol i (inr o) pt ->
+  exists pt1 pt2, reorder_pos pt (PINode pt1 o i pt2).
+Proof.
+  intros.
+  induction pt; inv H.
+  - eexists. eexists. eapply rtc_refl.
+  - apply IHpt1 in H2.
+    destruct H2. destruct H.
+    eexists. eexists.
+    eapply rtc_transitive.
+    + eapply reorder_pos_subtree_l.
+      eassumption.
+    + eapply rtc_once.
+      eapply PRI_LR.
+  - apply IHpt2 in H2.
+    destruct H2. destruct H.
+    eexists. eexists.
+    eapply rtc_transitive.
+    + eapply reorder_pos_subtree_r.
+      eassumption.
+    + eapply rtc_once.
+      eapply PRI_RL.
+Qed.
+
+Lemma pos_equivalent_reorder_pos pt1 pt2 n0 n :
+  wf_pos_tree n0 pt1 n -> wf_pos_tree n0 pt2 n ->    
+  pos_equivalent pt1 pt2 ->
+  reorder_pos pt1 pt2.
+Proof.
+  intro. revert pt2.
+  induction H.
+
+  - intros.
+    unfold pos_equivalent in H0.
+    destruct pt2.
+    + specialize H0 with (s := inl l) (i0 := i).
+      destruct H0.
+      assert (@nth_symbol L O i (inl l) (PANode l i)). apply L_nth.
+      apply H0 in H2.
+      inv H2.
+      apply rtc_refl.
+    + specialize H0 with (s := inr o) (i0 := n).
+      destruct H0.
+      assert (nth_symbol n (inr o) (PINode pt2_1 o n pt2_2)). apply O_nth.
+      apply H1 in H2.
+      inv H2.
+
+  - intros.
+
+    assert (H2' := H2).
+    unfold pos_equivalent in H2'.
+    specialize H2' with (s := inr o) (i := j).
+    assert (nth_symbol j (inr o) (PINode pt1 o j pt2)). apply O_nth.
+    apply H2' in H3. clear H2'.
+
+    apply reorder_pos_nth_op_top in H3.
+    destruct H3.
+    destruct H3.
+    eapply reorder_pos_wf_pos_tree in H3 as ?; eauto.
+    inv H4.
+    eapply reorder_pos_preserves_position in H3 as ?; eauto.
+    assert (pos_equivalent (PINode pt1 o j pt2) (PINode x o j x0)). {
+      eapply pos_equivalent_transitive; eassumption.
+    }
+    eapply pos_equivalent_subtrees in H5; eauto with pos_tree.
+    destruct H5.
+    apply IHwf_pos_tree1 in H5; auto.
+    apply IHwf_pos_tree2 in H6; auto.
+    eapply rtc_transitive.
+    eapply reorder_pos_subtree_l.
+    eassumption.
+    eapply rtc_transitive.
+    eapply reorder_pos_subtree_r.
+    eassumption.
+    apply reorder_pos_symmetry.
+    assumption.
+Qed.
+
+Lemma reorder_step_pos_unpos_reorder_step pt pt' :
+  reorder_step_pos pt pt' -> reorder_step (unpos pt) (unpos pt').
+Proof.
+  intros.
+  induction H; simpl.
+  - apply RI_LR.
+  - apply RI_RL.
+  - apply RI_t1. assumption.
+  - apply RI_t2. assumption.
+Qed.
+
+Lemma reorder_pos_unpos_reorder pt pt' :
+  reorder_pos pt pt' -> reorder (unpos pt) (unpos pt').
+Proof.
+  intros.
+  induction H.
+  - apply rtc_refl.
+  - eapply rtc_l.
+    + apply reorder_step_pos_unpos_reorder_step.
+      eassumption.
+    + assumption.
+Qed.
+
+Lemma reorder_pos_forall_unpos :
+  (forall pt pt' n0 n,
+    wf_pos_tree n0 pt n -> wf_pos_tree n0 pt' n ->
+    pos_equivalent pt pt' -> reorder_pos pt pt') ->
+  (forall t t', yield t = yield t' -> reorder t t').
+Proof.
+  intros.
+
+  remember (pos t 0) as x.
+  destruct x.
+  symmetry in Heqx.
+  apply pos_unpos in Heqx as ?.
+  apply pos_wf_pos_tree in Heqx as ?.
+  remember (pos t' 0) as x'.
+  destruct x'.
+  symmetry in Heqx'.
+  apply pos_unpos in Heqx' as ?.
+  apply pos_wf_pos_tree in Heqx' as ?.
+  apply wf_pos_tree_size in H4 as ?.
+  apply wf_pos_tree_size in H2 as ?.
+  simpl in *. subst.
+  rewrite H0 in H2.
+  eapply pos_equivalence_yields in H0; eauto.
+  apply reorder_pos_unpos_reorder.
+  eapply H; eauto.
+Qed.
+
+Lemma reorder_completes_yields t t' :
+  yield t = yield t' -> reorder t t'.
+Proof.
+  apply reorder_pos_forall_unpos.
+  apply pos_equivalent_reorder_pos.
+Qed.
+
+Theorem yield_equivalence_are_reorderings t t' :
+  yield t = yield t' <-> reorder t t'.
+Proof.
+  split.
+  - apply reorder_completes_yields.
+  - apply reorder_preserves_yield.
+Qed.
+
+
